\chapter{演示}
\vspace{7pt}
\section{公式演示}
\begin{equation}
	\ppx{y}, \ppx[y]{w}
\end{equation}

\begin{equation}
	\begin{split}
		&\ppx{u}+\ppx[y]{v}+\ppx[z]{w}=0\\
		&\ma A=\ma S+\ma O\\
		&\dt{\ve n}=\ma A \cdot \ve n
	\end{split}
\end{equation}

\begin{equation}
	\ma I'=\frac{1}{5}m_p\left[\begin{matrix}
		2b^2&0&0\\
		0&a^2+b^2&0\\
		0&0&a^2+b^2
	\end{matrix}\right],
\end{equation}

\newcommand\Stt{\widetilde{St_r}}
\newcommand{\Stc}{St_r C_\perp}
\newcommand{\Stcp}{St_r C_\parallel}
\newcommand{\halfof}[1]{\frac{#1}{2}}
\newcommand{\uhs}{\hat{\ve u}_s}
\newcommand{\kc}{k_\perp}
\newcommand{\kp}{k_\parallel}
\newcommand{\chic}{\chi_\perp}
\newcommand{\chip}{\chi_\parallel}

\begin{equation}
	\begin{split}
		T'_{J x} &=\frac{16\pi\mu b^3}{3\chic}(\Omega^{*\prime}_x-\omega^{*\prime}_x),\\
		T'_{J y} &=\frac{16\pi\mu b^3}{3(\lambda^2\chip+\chic)}[(1-\lambda^2)S^{*\prime}_{xz}+(1+\lambda^2)(\Omega^{*\prime}_y-\omega^{*\prime}_y)],\\
		T'_{J z} &=\frac{16\pi\mu b^3}{3(\lambda^2\chip+\chic)}[(\lambda^2-1)S^{*\prime}_{xy}+(\lambda^2+1)(\Omega^{*\prime}_z-\omega^{*\prime}_z)].
	\end{split}
\end{equation}

\begin{equation}
	\dt{}\left[\begin{matrix}
		\delta n_x\\\delta n_y\\
	\end{matrix}\right]=\left[\begin{matrix}
		\halfof{(-\Lambda^2-2M^2+\Lambda)\Stt}+M & -\halfof{(1+\Lambda)(M\Stt-1)}\\
		-\halfof{1}+\halfof{\Lambda}&0\\
	\end{matrix}\right]\left[\begin{matrix}
		\delta n_x\\\delta n_y\\
	\end{matrix}\right].
\end{equation}